Unify Curve and Ed

code/curve25519/Hacl.Spec.Curve25519.Field64.Core.fst
@@ -87,53 +87,54 @@ let add0carry x y =
   let c = if lt_u64 res x then u64 1 else u64 0 in
   res, c
 
-let carry_felem4 = uint64 & uint64 & uint64 & uint64 & uint64
 
-inline_for_extraction noextract
 val add1:
     f:felem4
   -> cin:uint64
-  -> Pure carry_felem4
+  -> Pure (uint64 & felem4)
     (requires True)
-    (ensures fun (c, r0, r1, r2, r3) ->
-      as_nat4 (r0, r1, r2, r3) + v c * pow2 256 == as_nat4 f + v cin)
-let add1 (f0, f1, f2, f3) cin =
+    (ensures fun (c, r) ->
+      as_nat4 r + v c * pow2 256 == as_nat4 f + v cin)
+let add1 f cin =
+  let (f0, f1, f2, f3) = f in
   let o0, c0 = add0carry f0 cin in
   let o1, c1 = add0carry f1 c0 in
   let o2, c2 = add0carry f2 c1 in
   let o3, c3 = add0carry f3 c2 in
+  let out = (o0, o1, o2, o3) in
   lemma_mul_assos_5 (v c3) (pow2 64) (pow2 64) (pow2 64) (pow2 64);
   assert_norm (pow2 64 * pow2 64 * pow2 64 * pow2 64 = pow2 256);
-  (c3, o0, o1, o2, o3)
+  c3, out
 
-inline_for_extraction noextract
 val sub1:
     f:felem4
   -> cin:uint64
-  -> Pure carry_felem4
+  -> Pure (uint64 & felem4)
     (requires True)
-    (ensures fun (c, r0, r1, r2, r3) ->
-      as_nat4 (r0, r1, r2, r3) - v c * pow2 256 == as_nat4 f - v cin)
-let sub1 (f0, f1, f2, f3) cin =
+    (ensures fun (c, r) ->
+      as_nat4 r - v c * pow2 256 == as_nat4 f - v cin)
+let sub1 f cin =
+  let (f0, f1, f2, f3) = f in
   let o0, c0 = subborrow f0 cin (u64 0) in
   let o1, c1 = subborrow f1 (u64 0) c0 in
   let o2, c2 = subborrow f2 (u64 0) c1 in
   let o3, c3 = subborrow f3 (u64 0) c2 in
+  let out = (o0, o1, o2, o3) in
   lemma_mul_assos_5 (v c3) (pow2 64) (pow2 64) (pow2 64) (pow2 64);
   assert_norm (pow2 64 * pow2 64 * pow2 64 * pow2 64 = pow2 256);
-  (c3, o0, o1, o2, o3)
+  c3, out
 
 #set-options "--z3rlimit 150"
 
-inline_for_extraction noextract
 val mul1:
     f:felem4
   -> u:uint64
-  -> Pure carry_felem4
+  -> Pure (uint64 & felem4)
     (requires True)
-    (ensures fun (c, r0, r1, r2, r3) ->
-      as_nat4 (r0, r1, r2, r3) + v c * pow2 256 == as_nat4 f * v u)
-let mul1 (f0, f1, f2, f3) u =
+    (ensures fun (c, r) ->
+      as_nat4 r + v c * pow2 256 == as_nat4 f * v u)
+let mul1 f u =
+  let (f0, f1, f2, f3) = f in
   let l0, h0 = mul64 f0 u in
   let l1, h1 = mul64 f1 u in
   let l2, h2 = mul64 f2 u in
@@ -157,8 +158,6 @@ let mul1 (f0, f1, f2, f3) u =
     v f3 * v u * pow2 64 * pow2 64 * pow2 64 -
     v h3 * pow2 64 * pow2 64 * pow2 64 * pow2 64 -
     v c2 * pow2 64 * pow2 64 * pow2 64 * pow2 64);
-
-  let f = (f0, f1, f2, f3) in
   lemma_mul1_simplify out f u h3 c2;
   assert (as_nat4 out + (v h3 + v c2) * pow2 256 == as_nat4 f * v u);
 
@@ -166,25 +165,22 @@ let mul1 (f0, f1, f2, f3) u =
   lemma_as_nat4 out;
   lemma_mul1_no_carry (as_nat4 out) (as_nat4 f * v u) (v h3 + v c2);
   let c3 = h3 +! c2 in
-  (c3, o0, o1, o2, o3)
+  c3, out
 
-inline_for_extraction noextract
 val mul1_add:
     f1:felem4
   -> u2:uint64
   -> f3:felem4
-  -> Pure carry_felem4
+  -> Pure (uint64 & felem4)
     (requires True)
-    (ensures fun (c, r0, r1, r2, r3) ->
-      as_nat4 (r0, r1, r2, r3) + v c * pow2 256 == as_nat4 f3 + as_nat4 f1 * v u2)
-let mul1_add (f10, f11, f12, f13) u2 (f30, f31, f32, f33) =
-  let f1 = (f10, f11, f12, f13) in
-  let f3 = (f30, f31, f32, f33) in
+    (ensures fun (c, r) ->
+      as_nat4 r + v c * pow2 256 == as_nat4 f3 + as_nat4 f1 * v u2)
+let mul1_add f1 u2 f3 =
   lemma_mul1_add_pre f1 u2 f3;
   assert (as_nat4 f3 + as_nat4 f1 * v u2 < pow2 320);
-  let c, o0, o1, o2, o3 = mul1 f1 u2 in
-  let out0 = (o0, o1, o2, o3) in
-
+  let c, out0 = mul1 f1 u2 in
+  let (o0, o1, o2, o3) = out0 in
+  let (f30, f31, f32, f33) = f3 in
   let o0', c0 = addcarry f30 o0 (u64 0) in
   let o1', c1 = addcarry f31 o1 c0 in
   let o2', c2 = addcarry f32 o2 c1 in
@@ -205,21 +201,20 @@ let mul1_add (f10, f11, f12, f13) u2 (f30, f31, f32, f33) =
   lemma_as_nat4 f3;
   lemma_mul1_add_no_carry (as_nat4 out) (as_nat4 f3) (as_nat4 f1) (v u2) (v c + v c3);
   let c4 = c +! c3 in
-  (c4, o0', o1', o2', o3')
+  c4, out
 
-inline_for_extraction noextract
 val carry_pass:
     f:felem4
   -> cin:uint64{v cin * 38 < pow2 63}
   -> out:felem4{feval out == (as_nat4 f + v cin * pow2 256) % prime}
 let carry_pass f cin =
   lemma_mul_pow256_add f cin;
-  let carry, o0, o1, o2, o3 = add1 f (cin *! u64 38) in
-  lemma_mul_pow256_add (o0, o1, o2, o3) carry;
+  let carry, out0 = add1 f (cin *! u64 38) in
+  let (o0, o1, o2, o3) = out0 in
+  lemma_mul_pow256_add out0 carry;
   let o0' = o0 +! carry *! u64 38 in
   (o0', o1, o2, o3)
 
-inline_for_extraction noextract
 val carry_wide:
     f:felem_wide4
   -> out:felem4{feval out == feval_wide f}
@@ -231,8 +226,7 @@ let carry_wide f =
   assert_norm (pow2 6 * pow2 256 = pow2 262);
   assert (as_nat4 (f0, f1, f2, f3) + as_nat4 (f4, f5, f6, f7) * 38 < pow2 263);
   assert_norm (pow2 263 < pow2 320);
-  let c0, o0, o1, o2, o3 = mul1_add (f4, f5, f6, f7) (u64 38) (f0, f1, f2, f3) in
-  let out0 = (o0, o1, o2, o3) in
+  let c0, out0 = mul1_add (f4, f5, f6, f7) (u64 38) (f0, f1, f2, f3) in
   assert (as_nat4 out0 + v c0 * pow2 256 == as_nat4 (f0, f1, f2, f3) + as_nat4 (f4, f5, f6, f7) * 38);
   lemma_as_nat4 out0;
   lemma_carry_wide (as_nat4 out0) (as_nat4 (f0, f1, f2, f3) + as_nat4 (f4, f5, f6, f7) * 38) (v c0);
@@ -240,62 +234,64 @@ let carry_wide f =
   lemma_feval_wide f;
   out1
 
-inline_for_extraction noextract
 val add4:
     f1:felem4
   -> f2:felem4
-  -> Pure carry_felem4
+  -> Pure (uint64 & felem4)
     (requires True)
-    (ensures fun (c, r0, r1, r2, r3) -> v c <= 1 /\
-      as_nat4 (r0, r1, r2, r3) + v c * pow2 256 == as_nat4 f1 + as_nat4 f2)
-let add4 (f10, f11, f12, f13) (f20, f21, f22, f23) =
+    (ensures fun (c, r) -> v c <= 1 /\
+      as_nat4 r + v c * pow2 256 == as_nat4 f1 + as_nat4 f2)
+let add4 f1 f2 =
+  let (f10, f11, f12, f13) = f1 in
+  let (f20, f21, f22, f23) = f2 in
   let o0, c0 = addcarry f10 f20 (u64 0) in
   let o1, c1 = addcarry f11 f21 c0 in
   let o2, c2 = addcarry f12 f22 c1 in
   let o3, c3 = addcarry f13 f23 c2 in
+  let out = (o0, o1, o2, o3) in
   lemma_mul_assos_5 (v c3) (pow2 64) (pow2 64) (pow2 64) (pow2 64);
   assert_norm (pow2 64 * pow2 64 * pow2 64 * pow2 64 = pow2 256);
-  (c3, o0, o1, o2, o3)
+  c3, out
 
-inline_for_extraction noextract
 val fadd4:
     f1:felem4
   -> f2:felem4
   -> out:felem4{feval out == fadd (feval f1) (feval f2)}
 let fadd4 f1 f2 =
-  let c0, o0, o1, o2, o3 = add4 f1 f2 in
-  let out = carry_pass (o0, o1, o2, o3) c0 in
+  let c0, out0 = add4 f1 f2 in
+  let out = carry_pass out0 c0 in
   assert (feval out == (as_nat4 f1 + as_nat4 f2) % prime);
   FStar.Math.Lemmas.lemma_mod_plus_distr_l (as_nat4 f1) (as_nat4 f2) prime;
   FStar.Math.Lemmas.lemma_mod_plus_distr_r ((as_nat4 f1) % prime) (as_nat4 f2) prime;
   out
 
-inline_for_extraction noextract
 val sub4:
     f1:felem4
   -> f2:felem4
-  -> Pure carry_felem4
+  -> Pure (uint64 & felem4)
     (requires True)
-    (ensures fun (c, r0, r1, r2, r3) -> v c <= 1 /\
-      as_nat4 (r0, r1, r2, r3) - v c * pow2 256 == as_nat4 f1 - as_nat4 f2)
-let sub4 (f10, f11, f12, f13) (f20, f21, f22, f23) =
+    (ensures fun (c, r) -> v c <= 1 /\
+      as_nat4 r - v c * pow2 256 == as_nat4 f1 - as_nat4 f2)
+let sub4 f1 f2 =
+  let (f10, f11, f12, f13) = f1 in
+  let (f20, f21, f22, f23) = f2 in
   let o0, c0 = subborrow f10 f20 (u64 0) in
   let o1, c1 = subborrow f11 f21 c0 in
   let o2, c2 = subborrow f12 f22 c1 in
   let o3, c3 = subborrow f13 f23 c2 in
+  let out = (o0, o1, o2, o3) in
   lemma_mul_assos_5 (v c3) (pow2 64) (pow2 64) (pow2 64) (pow2 64);
   assert_norm (pow2 64 * pow2 64 * pow2 64 * pow2 64 = pow2 256);
-  (c3, o0, o1, o2, o3)
+  c3, out
 
-inline_for_extraction noextract
 val fsub4:
     f1:felem4
   -> f2:felem4
   -> out:felem4{feval out == fsub (feval f1) (feval f2)}
 let fsub4 f1 f2 =
-  let c0, o00, o01, o02, o03 = sub4 f1 f2 in
-  let c1, o0, o1, o2, o3 = sub1 (o00, o01, o02, o03) (c0 *! u64 38) in
-  let out1 = (o0, o1, o2, o3) in
+  let c0, out0 = sub4 f1 f2 in
+  let c1, out1 = sub1 out0 (c0 *! u64 38) in
+  let (o0, o1, o2, o3) = out1 in
   let o0' = o0 -! c1 *! u64 38 in
   let out2 = (o0', o1, o2, o3) in
   assert (as_nat4 out2 == as_nat4 out1 - v c1 * 38);
@@ -304,23 +300,27 @@ let fsub4 f1 f2 =
   lemma_fsub4 out2 f1 f2 c0 c1;
   out2
 
-inline_for_extraction noextract
 val mul4:
     f:felem4
   -> r:felem4
   -> out:felem_wide4{wide_as_nat4 out == as_nat4 f * as_nat4 r}
-let mul4 (f0, f1, f2, f3) r =
-  let c0, o00, o01, o02, o03 = mul1 r f0 in
-  let c1, o11, o12, o13, o14 = mul1_add r f1 (o01, o02, o03, c0) in
-  let c2, o22, o23, o24, o25 = mul1_add r f2 (o12, o13, o14, c1) in
-  let c3, o33, o34, o35, o36 = mul1_add r f3 (o23, o24, o25, c2) in
+let mul4 f r =
+  let (f0, f1, f2, f3) = f in
+  let c0, out0 = mul1 r f0 in
+  let (o00, o01, o02, o03) = out0 in
+  let c1, out1 = mul1_add r f1 (o01, o02, o03, c0) in
+  let (o11, o12, o13, o14) = out1 in
+  let c2, out2 = mul1_add r f2 (o12, o13, o14, c1) in
+  let (o22, o23, o24, o25) = out2 in
+  let c3, out3 = mul1_add r f3 (o23, o24, o25, c2) in
+  let (o33, o34, o35, o36) = out3 in
   let o37 = c3 in
+  let out = (o00, o11, o22, o33, o34, o35, o36, o37) in
   lemma_mul4 (as_nat4 r) (v f0) (v f1) (v f2) (v f3) (v c0) (v c1) (v c2) (v c3)
     (v o01) (v o02) (v o03) (v o12) (v o13) (v o14) (v o23) (v o24) (v o25) (v o34) (v o35) (v o36);
-  lemma_mul4_expand (f0, f1, f2, f3) r;
-  (o00, o11, o22, o33, o34, o35, o36, o37)
+  lemma_mul4_expand f r;
+  out
 
-inline_for_extraction noextract
 val fmul4:
     f1:felem4
   -> r:felem4
@@ -332,14 +332,12 @@ let fmul4 f1 r =
   FStar.Math.Lemmas.lemma_mod_mul_distr_r (as_nat4 f1 % prime) (as_nat4 r) prime;
   out
 
-inline_for_extraction noextract
 val fmul14:
     f1:felem4
   -> f2:uint64{v f2 < pow2 17} //121665 < pow2 17
   -> out:felem4{feval out == (feval f1 * v f2) % prime}
 let fmul14 f1 f2 =
-  let c0, o0, o1, o2, o3 = mul1 f1 f2 in
-  let out0 = (o0, o1, o2, o3) in
+  let c0, out0 = mul1 f1 f2 in
   assert (as_nat4 out0 + v c0 * pow2 256 == as_nat4 f1 * v f2);
   lemma_as_nat4 f1;
   lemma_fmul14 (as_nat4 f1) (v f2);
@@ -351,3 +349,14 @@ let fmul14 f1 f2 =
   assert (feval out1 == (as_nat4 f1 * v f2) % prime);
   FStar.Math.Lemmas.lemma_mod_mul_distr_l (as_nat4 f1) (v f2) prime;
   out1
+
+val sqr4: f:felem4 -> out:felem_wide4{wide_as_nat4 out == as_nat4 f * as_nat4 f}
+let sqr4 f = mul4 f f
+
+val fsqr4: f:felem4 -> out:felem4{feval out == fmul (feval f) (feval f)}
+let fsqr4 f =
+  let tmp = sqr4 f in
+  let out = carry_wide tmp in
+  FStar.Math.Lemmas.lemma_mod_mul_distr_l (as_nat4 f) (as_nat4 f) prime;
+  FStar.Math.Lemmas.lemma_mod_mul_distr_r (as_nat4 f % prime) (as_nat4 f) prime;
+  out
