code/curve25519/Hacl.Impl.Curve25519.AddAndDouble.fst
@@ -18,7 +18,7 @@ module F64 = Hacl.Impl.Curve25519.Field64
 module P = Spec.Curve25519
 module S = Hacl.Spec.Curve25519.AddAndDouble
 
-#reset-options "--z3rlimit 150 --max_fuel 1 --using_facts_from '* -FStar.Seq'"
+#reset-options "--z3rlimit 150 --max_fuel 1 --using_facts_from '* -FStar.Seq' --record_options"
 
 inline_for_extraction noextract
 let point (s:field_spec) = lbuffer (limb s) (nlimb s +! nlimb s)
@@ -49,7 +49,6 @@ let point_post_add_t #s h f =
   | M51 -> F51.felem_fits h f (2, 4, 2, 2, 2)
   | M64 -> True
 
-inline_for_extraction noextract
 val point_add_and_double0:
     #s:field_spec
   -> nq_p1:point s
@@ -58,6 +57,7 @@ val point_add_and_double0:
   -> tmp2:felem_wide2 s
   -> Stack unit
     (requires fun h0 ->
+      (s = M64 ==> Vale.X64.CPU_Features_s.(adx_enabled /\ bmi2_enabled)) /\
       live h0 nq_p1 /\ live h0 ab /\ live h0 dc /\ live h0 tmp2 /\
       disjoint nq_p1 ab /\ disjoint nq_p1 dc /\ disjoint nq_p1 tmp2 /\
       disjoint ab dc /\ disjoint ab tmp2 /\ disjoint dc tmp2 /\
@@ -68,6 +68,7 @@ val point_add_and_double0:
       modifies (loc nq_p1 |+| loc dc |+| loc tmp2) h0 h1 /\
       point_post_add_t h1 (get_x nq_p1) /\ point_post_sub_t h1 (get_z nq_p1) /\
       fget_xz h1 nq_p1 == S.add_and_double1_0 (fget_x h0 ab) (fget_z h0 ab) (fget_xz h0 nq_p1))
+[@ Meta.Attribute.inline_ ]
 let point_add_and_double0 #s nq_p1 ab dc tmp2 =
   let x3 = sub nq_p1 0ul (nlimb s) in
   let z3 = sub nq_p1 (nlimb s) (nlimb s) in
@@ -86,7 +87,6 @@ let point_add_and_double0 #s nq_p1 ab dc tmp2 =
   fadd x3 d c;  // x3 = da + cb
   fsub z3 d c  // z3 = da - cb
 
-inline_for_extraction noextract
 val point_add_and_double1:
     #s:field_spec
   -> nq:point s
@@ -95,6 +95,7 @@ val point_add_and_double1:
   -> tmp2:felem_wide2 s
   -> Stack unit
     (requires fun h0 ->
+      (s = M64 ==> Vale.X64.CPU_Features_s.(adx_enabled /\ bmi2_enabled)) /\
       live h0 nq /\ live h0 nq_p1 /\ live h0 tmp1 /\ live h0 tmp2 /\
       disjoint nq nq_p1 /\ disjoint nq tmp1 /\ disjoint nq tmp2 /\
       disjoint nq_p1 tmp1 /\ disjoint nq_p1 tmp2 /\ disjoint tmp1 tmp2 /\
@@ -109,6 +110,7 @@ val point_add_and_double1:
       (fget_xz h1 nq, fget_xz h1 nq_p1) ==
 	S.add_and_double1_1 (feval h0 (gsub tmp1 0ul (nlimb s)))
 	  (feval h0 (gsub tmp1 (nlimb s) (nlimb s))) (fget_xz h0 nq_p1))
+[@ Meta.Attribute.inline_ ]
 let point_add_and_double1 #s nq nq_p1 tmp1 tmp2 =
   let x2 = sub nq 0ul (nlimb s) in
   let z2 = sub nq (nlimb s) (nlimb s) in
@@ -142,14 +144,15 @@ let point_add_and_double1 #s nq nq_p1 tmp1 tmp2 =
   //fmul z2 c b;  // z2 = e * (aa + (e * 121665))
   fmul2 nq dc ab tmp2  // x2|z2 = aa * bb | e * (aa + (e * 121665))
 
-inline_for_extraction noextract
-val point_add_and_double_:
+val point_add_and_double:
     #s:field_spec
   -> q:point s
   -> p01_tmp1:lbuffer (limb s) (8ul *! nlimb s)
   -> tmp2:felem_wide2 s
   -> Stack unit
-    (requires fun h0 -> (
+    (requires fun h0 ->
+      (s = M64 ==> Vale.X64.CPU_Features_s.(adx_enabled /\ bmi2_enabled)) /\
+    (
       let nq = gsub p01_tmp1 0ul (2ul *! nlimb s) in
       let nq_p1 = gsub p01_tmp1 (2ul *! nlimb s) (2ul *! nlimb s) in
       live h0 q /\ live h0 p01_tmp1 /\ live h0 tmp2 /\
@@ -165,7 +168,8 @@ val point_add_and_double_:
       state_inv_t h1 (get_x nq_p1) /\ state_inv_t h1 (get_z nq_p1) /\
      (let p2, p3 = P.add_and_double (fget_xz h0 q) (fget_xz h0 nq) (fget_xz h0 nq_p1) in
       fget_xz h1 nq == p2 /\ fget_xz h1 nq_p1 == p3)))
-let point_add_and_double_ #s q p01_tmp1 tmp2 =
+[@ Meta.Attribute.specialize ]
+let point_add_and_double #s q p01_tmp1 tmp2 =
   let h0 = ST.get () in
   let nq : point s = sub p01_tmp1 0ul (2ul *! nlimb s) in
   let nq_p1 : point s = sub p01_tmp1 (2ul *! nlimb s) (2ul *! nlimb s) in
@@ -189,50 +193,14 @@ let point_add_and_double_ #s q p01_tmp1 tmp2 =
   fmul z3 z3 x1 tmp2; // z3 = x1 * (da - cb) ^ 2
   S.lemma_add_and_double (fget_xz h0 q) (fget_xz h0 nq) (fget_xz h0 nq_p1)
 
-(* WRAPPER to Prevent Inlining *)
-[@CInline]
-let point_add_and_double_51 (q:point51) (p01_tmp1:lbuffer uint64 40ul) = point_add_and_double_ #M51 q p01_tmp1
-[@CInline]
-let point_add_and_double_64 (q:point64) (p01_tmp1:lbuffer uint64 32ul) = point_add_and_double_ #M64 q p01_tmp1
-
-inline_for_extraction noextract
-val point_add_and_double:
-    #s:field_spec
-  -> q:point s
-  -> p01_tmp1:lbuffer (limb s) (8ul *! nlimb s)
-  -> tmp2:felem_wide2 s
-  -> Stack unit
-    (requires fun h0 -> (
-      let nq = gsub p01_tmp1 0ul (2ul *! nlimb s) in
-      let nq_p1 = gsub p01_tmp1 (2ul *! nlimb s) (2ul *! nlimb s) in
-      live h0 q /\ live h0 p01_tmp1 /\ live h0 tmp2 /\
-      disjoint q p01_tmp1 /\ disjoint q tmp2 /\ disjoint p01_tmp1 tmp2 /\
-      state_inv_t h0 (get_x q) /\ state_inv_t h0 (get_z q) /\
-      state_inv_t h0 (get_x nq) /\ state_inv_t h0 (get_z nq) /\
-      state_inv_t h0 (get_x nq_p1) /\ state_inv_t h0 (get_z nq_p1)))
-    (ensures  fun h0 _ h1 -> (
-      let nq = gsub p01_tmp1 0ul (2ul *! nlimb s) in
-      let nq_p1 = gsub p01_tmp1 (2ul *! nlimb s) (2ul *! nlimb s) in
-      modifies (loc p01_tmp1 |+| loc tmp2) h0 h1 /\
-      state_inv_t h1 (get_x nq) /\ state_inv_t h1 (get_z nq) /\
-      state_inv_t h1 (get_x nq_p1) /\ state_inv_t h1 (get_z nq_p1) /\
-     (let p2, p3 = P.add_and_double (fget_xz h0 q) (fget_xz h0 nq) (fget_xz h0 nq_p1) in
-      fget_xz h1 nq == p2 /\ fget_xz h1 nq_p1 == p3)))
-let point_add_and_double #s q p01_tmp1 tmp2 =
-  match s with
-  | M51 -> point_add_and_double_51 q p01_tmp1 tmp2
-  | M64 -> point_add_and_double_64 q p01_tmp1 tmp2
-(* WRAPPER to Prevent Inlining *)
-
-
-inline_for_extraction noextract
-val point_double_:
+val point_double:
     #s:field_spec
   -> nq:point s
   -> tmp1:lbuffer (limb s) (4ul *! nlimb s)
   -> tmp2:felem_wide2 s
   -> Stack unit
     (requires fun h0 ->
+      (s = M64 ==> Vale.X64.CPU_Features_s.(adx_enabled /\ bmi2_enabled)) /\
       live h0 nq /\ live h0 tmp1 /\ live h0 tmp2 /\
       disjoint nq tmp1 /\ disjoint nq tmp2 /\ disjoint tmp1 tmp2 /\
       state_inv_t h0 (get_x nq) /\ state_inv_t h0 (get_z nq))
@@ -240,7 +208,8 @@ val point_double_:
       modifies (loc nq |+| loc tmp1 |+| loc tmp2) h0 h1 /\
       state_inv_t h1 (get_x nq) /\ state_inv_t h1 (get_z nq) /\
       fget_xz h1 nq == P.double (fget_xz h0 nq))
-let point_double_ #s nq tmp1 tmp2 =
+[@ Meta.Attribute.specialize ]
+let point_double #s nq tmp1 tmp2 =
   let x2 = sub nq 0ul (nlimb s) in
   let z2 = sub nq (nlimb s) (nlimb s) in
 
@@ -276,30 +245,3 @@ let point_double_ #s nq tmp1 tmp2 =
   //fmul x2 d a;  // x2 = aa * bb
   //fmul z2 c b;  // z2 = e * (aa + (e * 121665))
   fmul2 nq dc ab tmp2  // x2|z2 = aa * bb | e * (aa + (e * 121665))
-
-(* WRAPPER to Prevent Inlining *)
-[@CInline]
-let point_double_51 (nq:point51) = point_double_ #M51 nq
-[@CInline]
-let point_double_64 (nq:point64) = point_double_ #M64 nq
-
-inline_for_extraction noextract
-val point_double:
-    #s:field_spec
-  -> nq: point s
-  -> tmp1:lbuffer (limb s) (4ul *! nlimb s)
-  -> tmp2:felem_wide2 s
-  -> Stack unit
-    (requires fun h0 ->
-      live h0 nq /\ live h0 tmp1 /\ live h0 tmp2 /\
-      disjoint nq tmp1 /\ disjoint nq tmp2 /\ disjoint tmp1 tmp2 /\
-      state_inv_t h0 (get_x nq) /\ state_inv_t h0 (get_z nq))
-    (ensures  fun h0 _ h1 ->
-      modifies (loc nq |+| loc tmp1 |+| loc tmp2) h0 h1 /\
-      state_inv_t h1 (get_x nq) /\ state_inv_t h1 (get_z nq) /\
-      fget_xz h1 nq == P.double (fget_xz h0 nq))
-let point_double #s nq tmp1 tmp2 =
-  match s with
-  | M51 -> point_double_51 nq tmp1 tmp2
-  | M64 -> point_double_64 nq tmp1 tmp2
-(* WRAPPER to Prevent Inlining *)
